first draft of overall theorem

monadproofs/proofs/reservebal.v
@@ -48,10 +48,8 @@ Definition user_reserve_balance
  *)
 
 (* Predicate for “emptying transaction” – currently always returns false. *)
-Definition is_emptying_transaction
-  (sender : monad.proofs.evmopsem.evm.address)
-  (t0 : monad.proofs.evmopsem.Transaction)
-  : bool :=
+Definition tx_allowed_to_empty
+ (s : StateOfAccounts) (a : Transaction) : bool :=
   false.
 
 (*
@@ -66,6 +64,7 @@ Definition gas_limit_of (t : monad.proofs.evmopsem.Transaction) : N :=
     (monad.EVMOpSem.block.tr_gas_limit t).
 *)
 
+(* only gas fees. does not include value transfers *)
 Definition maxTxFee (s_n_minus_k: StateOfAccounts) (t: Transaction) : N. Proof. Admitted.
 
 (* Sum over gas_limit * gas_bid for a list of transactions. *)
@@ -78,23 +77,111 @@ Fixpoint sum_gas_bids (s_n_minus_k: StateOfAccounts) (l : list Transaction) : N 
 Definition staticReserveBal : N. Proof. Admitted.
 (* Consensus‐side acceptability check for sequencing [a], given state s = state^{n-k}
    and the list [intermediate] of prior txns from this sender after block n-k. *)
-Definition consensusAcceptableTx (s : StateOfAccounts) (intermediate : list Transaction) (a : Transaction) :=
+Definition consensusAcceptableTx (stateAfterLastExecuted : StateOfAccounts) (intermediate : list Transaction) (a : Transaction) :=
   let sender := block.tr_from a in
-  let bal0 := balanceOfAc s sender in
+  let bal0 := balanceOfAc stateAfterLastExecuted sender in
   match intermediate with
   | [] =>
       let reserve := staticReserveBal `min` bal0 in
-      bool_decide (maxTxFee s a ≤ reserve)
+      bool_decide (maxTxFee stateAfterLastExecuted a ≤ reserve)
   | t0 :: rest =>
-      if is_emptying_transaction sender t0
+      if tx_allowed_to_empty stateAfterLastExecuted t0
       then
-       let bal1 := bal0 - w256_to_N (block.tr_value t0) - maxTxFee s t0 in
+       let bal1 := bal0 - w256_to_N (block.tr_value t0) - maxTxFee stateAfterLastExecuted t0 in
        let reserve := staticReserveBal `min` bal1 in
-       bool_decide (sum_gas_bids s (a::rest) ≤ reserve)
+       bool_decide (sum_gas_bids stateAfterLastExecuted (a::rest) ≤ reserve)
       else
        let reserve := staticReserveBal `min` bal0 in
-       bool_decide (sum_gas_bids s (a::intermediate) ≤ reserve)
+       bool_decide (sum_gas_bids stateAfterLastExecuted (a::intermediate) ≤ reserve)
   end.
-    (* ----------------------------------------------------------------------- *)
 
+Fixpoint consensusAcceptableTxs (s : StateOfAccounts) (intermediateTxs ltx : list Transaction) : bool :=
+  match ltx with
+  | [] => true
+  | h::tl => consensusAcceptableTx s intermediateTxs h && consensusAcceptableTxs s (intermediateTxs++[h]) tl
+  end.
+    
+Definition consensusAcceptableBlocks (stateAfterLastExecuted : StateOfAccounts)
+  (proposedChainExtension: list Block) : bool :=
+  let allTx := flat_map transactions proposedChainExtension in
+  consensusAcceptableTxs stateAfterLastExecuted [] allTx.
+
+Definition stateAfterBlockV2 (b: Block) (s: StateOfAccounts): option (StateOfAccounts * list TransactionResult) :=
+  match stateAfterTransactionsV2 (header b) s (transactions b) with
+  | None => None
+  | Some (s, tr) =>
+      let s:= applyWithdrawals s (withdrawals b) in
+      Some (applyBlockReward s (length (ommers b)), tr)
+  end.
+
+Fixpoint stateAfterBlocks (stateAfterLastExecuted : StateOfAccounts)
+  (proposedChainExtension: list Block) :
+  option (StateOfAccounts * list (list TransactionResult)) :=
+  match proposedChainExtension with
+  | [] => Some (stateAfterLastExecuted, [])
+  | h::tl => match stateAfterBlockV2 h stateAfterLastExecuted with
+             | None => None
+             | Some (si, rcpts) =>
+                 match stateAfterBlocks si tl with
+                 | None => None
+                 | Some (sf, lrcpts) => Some (sf, rcpts::lrcpts)
+                 end
+             end
+  end.
+    
+               
+Lemma soundness (stateAfterLastExecuted : StateOfAccounts)
+  (proposedChainExtension: list Block) :
+  consensusAcceptableBlocks stateAfterLastExecuted proposedChainExtension = true
+  -> isSome (stateAfterBlocks stateAfterLastExecuted proposedChainExtension).
+Abort.
+
+Definition maxFeeHeader (lb: list Block) : BlockHeader. Proof. Admitted.
+
+
+Lemma execTxMono header (s1 s2 : StateOfAccounts) i (tx: Transaction) :
+  (forall addr, balanceOfAc s1 addr <= balanceOfAc s2 addr)
+  -> isSome (stateAfterTransactionV2 header i s1 tx)
+  -> isSome (stateAfterTransactionV2 header i s2 tx).
+Proof. Admitted.
+
+Lemma execTxsMono header (s1 s2 : StateOfAccounts) (ltx: list Transaction) :
+  (forall addr, balanceOfAc s1 addr <= balanceOfAc s2 addr)
+  -> isSome (stateAfterTransactionsV2 header s1 ltx)
+  -> isSome (stateAfterTransactionsV2 header s2 ltx).
+Proof. Admitted.
+
+
+Lemma execBlockAsTxs (stateAfterLastExecuted : StateOfAccounts)
+  (proposedChainExtension: list Block) :
+  isSome (stateAfterTransactionsV (maxFeeHeader proposedChainExtension) stateAfterLastExecuted
+            (flat_map transactions proposedChainExtension))
+         ->
+  isSome (stateAfterBlocks stateAfterLastExecuted proposedChainExtension).
+Proof using. Admitted.
+
+Lemma soundnessAsTx (stateAfterLastExecuted : StateOfAccounts)
+  (proposedChainExtension: list Block) (lt : list Transaction):
+  consensusAcceptableTxs stateAfterLastExecuted [] lt = true
+    → isSome (stateAfterTransactionsV (maxFeeHeader proposedChainExtension) stateAfterLastExecuted lt).
+Proof using. Admitted.
+
+Lemma soundness (stateAfterLastExecuted : StateOfAccounts)
+  (proposedChainExtension: list Block) :
+  consensusAcceptableBlocks stateAfterLastExecuted proposedChainExtension = true
+  -> isSome (stateAfterBlocks stateAfterLastExecuted proposedChainExtension).
+Proof using.
+  unfold consensusAcceptableBlocks.
+  intros Hp.
+  apply execBlockAsTxs.
+  apply soundnessAsTx.
+  assumption.
+Qed.    
+        
+        
+
+(*
+Questions:
+- what is maxHeader
+- why can 
 
